General fromADT Lemma!

lib/FromADT.v
@@ -25,6 +25,32 @@ Proof.
   apply PickComputes; reflexivity.
 Qed.
 
+Fixpoint annotate_Constructor
+         {oldRep}
+         (dom : list Type)
+         (P : oldRep -> Prop)
+         (newRep := { r : oldRep | P r }%type)
+         {struct dom}
+  : (constructorType oldRep dom)
+    -> (constructorType newRep dom) :=
+  match dom return
+        constructorType oldRep dom ->
+        constructorType _ dom
+  with
+  | nil => fun oldMeth v => oldMeth (` v)
+  | cons domT dom' =>
+    fun oldMeth d =>
+      annotate_Constructor dom' P (oldMeth d)
+  end.
+
+Definition annotate_ConsDef
+           {oldRep}
+           (Sig : consSig)
+           (oldCons : @consDef oldRep Sig)
+           (P : oldRep -> Prop)
+  : @consDef _ Sig :=
+  {| consBody := annotate_Constructor _ P (consBody oldCons) |}.
+
 Tactic Notation "apply" "constructor" "knowledge" "for" constr(meth) :=
   apply (fromADTConstructor _ meth _); simpl;
   repeat
@@ -64,6 +90,50 @@ Proof.
   apply BindComputes with (a:=x); trivial.
   apply PickComputes; reflexivity.
 Qed.
+
+Fixpoint annotate_Method'
+         {oldRep}
+         (dom : list Type)
+         (cod : option Type)
+         (P : oldRep -> Prop)
+         (newRep := { r : oldRep | P r }%type)
+         {struct dom}
+  : (methodType' oldRep dom cod)
+    -> (methodType' newRep dom cod) :=
+  match dom return
+        methodType' oldRep dom cod ->
+        methodType' _ dom cod
+  with
+  | nil =>
+    match cod return
+          methodType' oldRep nil cod ->
+          methodType' _ nil cod
+    with
+    | Some codT => fun oldMeth v => oldMeth (` (fst v), snd v)
+    | None => fun oldMeth v => oldMeth (`v)
+    end
+  | cons domT dom' =>
+    fun oldMeth d =>
+      annotate_Method' dom' cod P (oldMeth d)
+  end.
+
+Definition annotate_Method
+           {oldRep}
+           (dom : list Type)
+           (cod : option Type)
+           (oldMethod : methodType oldRep dom cod)
+           (P : oldRep -> Prop)
+           (newRep := { r : oldRep | P r }%type)
+  : methodType newRep dom cod :=
+  fun r => annotate_Method' dom cod P (oldMethod (` r)).
+
+Definition annotate_MethDef
+           {oldRep}
+           (Sig : methSig)
+           (oldCons : @methDef oldRep Sig)
+           (P : oldRep -> Prop)
+  : @methDef _ Sig :=
+  {| methBody := annotate_Method (methBody oldCons) P |}.
 
 Tactic Notation "apply" "method" "knowledge" "for"
        constr(S) constr(meth) constr(H) :=
@@ -105,6 +175,147 @@ Tactic Notation "annotate" constr(spec) "ADT" :=
        (fun (or : Rep spec)
             (nr : { r : Rep spec | fromADT spec r }) => or = ` nr);
   resolve_method_bodies.
+
+Definition refineMethod_w_PreCond
+           {oldRep newRep}
+           (AbsR : oldRep -> newRep -> Prop)
+           (P : oldRep -> Prop)
+           {dom : list Type}
+           {cod : option Type}
+           (oldMethod : methodType oldRep dom cod)
+           (newMethod : methodType newRep dom cod)
+  := forall r_o r_n,
+    P r_o
+    -> AbsR r_o r_n
+    -> @refineMethod' _ _ AbsR dom cod (oldMethod r_o) (newMethod r_n).
+
+Lemma refineMethod'_trans rep rep' rep'' Dom Cod
+      AbsR AbsR'
+  : forall m m' m'',
+    @refineMethod' rep rep' AbsR Dom Cod m m'
+    -> @refineMethod' rep' rep'' AbsR' Dom Cod m' m''
+    -> refineMethod' (fun r_o r_n => exists r_o', AbsR r_o r_o' /\ AbsR' r_o' r_n)
+                         m m''.
+Proof.
+  induction Dom.
+  - intro; simpl; intros; destruct Cod; subst; intros v Comp_v.
+    + destruct_ex; intuition.
+      eapply H0 in Comp_v; eauto; computes_to_inv; subst.
+      eapply H in Comp_v; eauto; computes_to_inv; subst; eauto.
+      repeat computes_to_econstructor; eauto.
+    + destruct_ex; intuition.
+      eapply H0 in Comp_v; eauto; computes_to_inv; subst.
+      eapply H in Comp_v; eauto; computes_to_inv; subst; eauto.
+  - simpl; intros.
+    destruct_ex; intuition.
+    eapply (IHDom (m d)
+                  (m' d)
+                  (m'' d)); eauto.
+Qed.
+
+Lemma refine_absConstructor_fromADT
+  : forall oldRep dom
+           (P : oldRep -> Prop)
+           (c : constructorType oldRep dom),
+    (forall r : oldRep, fromConstructor c r -> P r) ->
+    refineConstructor (fun (or : {r : oldRep | P r}) (nr : oldRep) => ` or = nr)
+                      (absConstructor (fun (or : oldRep) (nr : {r : oldRep | P r}) => or = ` nr) c) c.
+Proof.
+  induction dom.
+  - simpl; unfold refine; intros.
+    repeat computes_to_econstructor.
+    instantiate (1 := exist _ _ (H _ H0)).
+    eexists; split; eauto.
+    reflexivity.
+  - intros.
+    intro; eapply IHdom; intros; eauto.
+    eapply H.
+    eexists; eauto.
+Qed.
+
+Lemma refine_absMethod_fromADT
+  : forall oldRep dom cod
+           (P : oldRep -> Prop)
+           (c : methodType oldRep dom cod),
+    (forall r r' : oldRep, P r -> fromMethod c r r' -> P r') ->
+    forall r',
+    refineMethod' (fun (or : {r : oldRep | P r}) (nr : oldRep) => ` or = nr)
+                  (absMethod' (fun (or : oldRep) (nr : {r : oldRep | P r}) => or = ` nr) dom cod c r') (c (` r')).
+Proof.
+  unfold fromMethod.
+  induction dom.
+  - destruct cod; simpl; unfold refine; intros.
+    + destruct r'; destruct v.
+      repeat computes_to_econstructor; intros; subst; simpl in H0.
+      instantiate (1 := (exist _ _ ((H _ _ p (ex_intro (fun c0 => c x ↝ (_, c0)) _ H0))), _)); simpl.
+      eexists; split; eauto.
+      reflexivity.
+      computes_to_econstructor.
+    + destruct r'.
+      repeat computes_to_econstructor; intros; subst; simpl in H0.
+      instantiate (1 := exist _ _ ((H _ _ p H0))); simpl.
+      eexists; split; eauto.
+      reflexivity.
+  - simpl; intros; eapply IHdom; eauto.
+Qed.
+
+Lemma annotate_ADT
+      {oldRep newRep}
+      (AbsR : oldRep -> newRep -> Prop)
+      {n n'}
+      {consSigs : Vector.t consSig n}
+      {methSigs : Vector.t methSig n'}
+      (consDefs : ilist (B := @consDef oldRep) consSigs)
+      (consDefs' : ilist (B := @consDef newRep) consSigs)
+      (methDefs : ilist (B := @methDef oldRep) methSigs)
+      (methDefs' : ilist (B := @methDef newRep) methSigs)
+      (ConstructorsRefineSpec
+       : IterateBoundedIndex.Iterate_Dep_Type_BoundedIndex
+           (fun idx  =>
+              refineConstructor
+                AbsR
+                (dom := consDom (Vector.nth consSigs idx))
+                (getConsDef consDefs idx)
+                (getConsDef consDefs' idx)))
+      (MethodsRefineSpec
+       : IterateBoundedIndex.Iterate_Dep_Type_BoundedIndex
+           (fun idx  =>
+              refineMethod_w_PreCond
+                AbsR
+                (fromADT (BuildADT consDefs methDefs))
+                (dom := methDom (Vector.nth methSigs idx))
+                (getMethDef methDefs idx)
+                (getMethDef methDefs' idx)))
+  :
+  refineADT
+    (BuildADT consDefs methDefs)
+    (BuildADT consDefs' methDefs').
+Proof.
+  eapply transitivityT.
+  - apply refineADT_Build_ADT_Rep_default with
+    (AbsR := fun or (nr : { r : oldRep | fromADT (BuildADT consDefs methDefs) r }) =>
+               or = ` nr).
+  - eapply refinesADT; intros.
+    + simpl Constructors.
+      generalize (IterateBoundedIndex.Lookup_Iterate_Dep_Type _ ConstructorsRefineSpec idx) as refineCons'; clear; intros;
+      eapply refineConstructor_trans with
+      (AbsR := fun or nr => `or = nr)
+      (AbsR' := AbsR); eauto.
+      clear.
+      unfold getConsDef.
+      generalize (@fromADTConstructor _ (BuildADT consDefs methDefs) idx);
+        simpl Constructors.
+      eapply refine_absConstructor_fromADT.
+    + simpl Methods.
+      generalize (IterateBoundedIndex.Lookup_Iterate_Dep_Type _ MethodsRefineSpec idx) as refineMeth'; simpl; clear;
+        intros ? [r_o' fromADT_r_o] r_n [ r_o [eq_r_o AbsR_r_o] ];
+        simpl in *; subst.
+      specialize (refineMeth' _ _ (fromADT_r_o) AbsR_r_o).
+      eapply refineMethod'_trans; eauto.
+      eapply refine_absMethod_fromADT.
+      intros.
+      eapply fromADTMethod with (midx := idx); eauto.
+Qed.
 
 Lemma refine_strip_dependency :
   forall A (P : A -> Prop) x B (k : _ -> Comp B),
